fixing padding for cnot, adding matrices converter

FY/MatricesConverter.py
@@ -1,0 +1,77 @@
+import numpy as np
+from fractions import Fraction
+
+st = input("expression: ")
+name = input("name: ")
+
+I = np.eye(2)
+CNOT = np.array([[1, 0, 0, 0],
+                 [0, 1, 0, 0],
+                 [0, 0, 0, 1],
+                 [0, 0, 1, 0]])
+X = np.array([[0, 1],
+              [1, 0]])
+H = (1 / np.sqrt(2)) * np.array([[1, 1],
+                                 [1,-1]])
+Z = np.array([[1, 0],
+              [0, -1]])
+q0 = np.array([1, 0]).reshape(1, -1)
+q1 = np.array([0, 1]).reshape(1, -1)
+
+m0 = q0.T.dot(q0)
+m1 = q1.T.dot(q1)
+
+def parse(st):
+    mults = [s.strip() for s in st.split("×")]
+    exps = []
+    for m in mults:
+        exps.append(m.split("⊗"))
+    return mult_all(exps)
+
+def recur(exp):
+    if len(exp) == 0:
+        return 1
+    if "I 2" in exp[0]:
+        return np.kron(I, recur(exp[1:]))
+    if "X" in exp[0]:
+        return np.kron(X, recur(exp[1:]))
+    if "H" in exp[0]:
+        return np.kron(H, recur(exp[1:]))
+    if "Z" in exp[0]:
+        return np.kron(Z, recur(exp[1:]))
+    if "CNOT" in exp[0]:
+        return np.kron(CNOT, recur(exp[1:]))
+    if "∣0⟩⟨0∣" in exp[0]:
+        return np.kron(q0.T.dot(q0), recur(exp[1:]))
+    if "∣ 0 ⟩" in exp[0] or "∣0⟩" in exp[0]:
+        return np.kron(q0, recur(exp[1:]))
+    if "⟨ 0 ∣" in exp[0] or "⟨0∣" in exp[0]:
+        return np.kron(q0.T, recur(exp[1:]))
+
+def mult_all(exps):
+    if len(exps) == 1:
+        return recur(exps[0])
+    return recur(exps[0]).dot(mult_all(exps[1:]))
+
+def transform_matrix_to_coq_form(mat):
+    res = "l2M ["
+    for row in mat:
+        st = "["
+        for e in row:
+            st += str(Fraction("{:.1f}".format(e))) + ";"
+        st = st[:-1] + "];\n"
+        res += st
+    res = res[:-2] + "]"
+    return res
+
+def generate_lemma(st, name):
+    mat = parse(st)
+    lemma = """
+Lemma {}: {} = {}.
+Proof.
+(* BY PYTHON SCRIPT *)
+Admitted.
+""".format(name, st, transform_matrix_to_coq_form(mat))
+    return lemma
+    
+print(generate_lemma(st, name))
